Phi_Semantics/PhiSem_Mem_C.thy
@@ -23,11 +23,15 @@ section \<open>Basic \<phi>Types for Semantic Models\<close>
 
 subsection \<open>Coercion from Value Spec to Mem Spec\<close>
 
+declare [[\<phi>trace_reasoning = 3]]
+
 \<phi>type_def Mem_Coercion :: \<open>(VAL,'a) \<phi> \<Rightarrow> (mem_fic,'a) \<phi>\<close> ("\<m>\<e>\<m>-\<c>\<o>\<e>\<r>\<c>\<e> _" [81] 80)
   where \<open>Mem_Coercion T \<equiv> (o) (to_share o map_option discrete) o Map_of_Val \<Zcomp>\<^sub>f T\<close>
   deriving Basic
        and Functional_Transformation_Functor
        and Commutativity_Deriver
+
+thm Mem_Coercion.ToA_mapper
 
 \<phi>type_def Guided_Mem_Coercion :: \<open>TY \<Rightarrow> (VAL,'a) \<phi> \<Rightarrow> (mem_fic,'a) \<phi>\<close> ("\<m>\<e>\<m>-\<c>\<o>\<e>\<r>\<c>\<e>[_] _" [50,81] 80)
   where \<open>\<m>\<e>\<m>-\<c>\<o>\<e>\<r>\<c>\<e>[TY] T \<equiv> \<m>\<e>\<m>-\<c>\<o>\<e>\<r>\<c>\<e> T\<close>
@@ -391,6 +395,21 @@ consts \<A>_mem_coerce :: mode
 declare Guided_Mem_Coercion.elim_map[where \<phi>=\<open>\<lambda>x. x\<close>, simplified, \<phi>reason %mapToA_mem_coerce_end]
         Guided_Mem_Coercion.elim_reasoning(1)[\<phi>reason %ToA_mem_coerce_end]
         Guided_Mem_Coercion.intro_reasoning(2)[\<phi>reason %ToA_mem_coerce_end]
+
+lemma
+  \<open> \<m>\<a>\<p> g \<otimes>\<^sub>f r : \<m>\<e>\<m>-\<c>\<o>\<e>\<r>\<c>\<e>[TY\<^sub>U] U \<^emph>[C\<^sub>R] R \<mapsto> \<m>\<e>\<m>-\<c>\<o>\<e>\<r>\<c>\<e>[TY\<^sub>U'] U' \<^emph>[C\<^sub>R] R'
+    \<o>\<v>\<e>\<r> f : \<m>\<e>\<m>-\<c>\<o>\<e>\<r>\<c>\<e>[TY] T \<^emph>[C\<^sub>W] W \<mapsto> T' \<^emph>[C\<^sub>W] W'
+    \<w>\<i>\<t>\<h> \<g>\<e>\<t>\<t>\<e>\<r> h \<s>\<e>\<t>\<t>\<e>\<r> s \<i>\<n> D
+\<Longrightarrow> \<m>\<a>\<p> g \<otimes>\<^sub>f r : \<m>\<e>\<m>-\<c>\<o>\<e>\<r>\<c>\<e>[TY\<^sub>U] U \<^emph>[C\<^sub>R] R \<mapsto> \<m>\<e>\<m>-\<c>\<o>\<e>\<r>\<c>\<e>[TY\<^sub>U'] U' \<^emph>[C\<^sub>R] R'
+    \<o>\<v>\<e>\<r> f : \<m>\<e>\<m>-\<c>\<o>\<e>\<r>\<c>\<e> T \<^emph>[C\<^sub>W] W \<mapsto> T' \<^emph>[C\<^sub>W] W'
+    \<w>\<i>\<t>\<h> \<g>\<e>\<t>\<t>\<e>\<r> h \<s>\<e>\<t>\<t>\<e>\<r> s \<i>\<n> D \<close>
+
+lemma
+  \<open> \<m>\<a>\<p> ?g \<otimes>\<^sub>f ?r : \<m>\<e>\<m>-\<c>\<o>\<e>\<r>\<c>\<e> ?Ta \<^emph>[?C\<^sub>R] ?R \<mapsto> \<m>\<e>\<m>-\<c>\<o>\<e>\<r>\<c>\<e> ?Tb \<^emph>[?C\<^sub>R] ?R' \<o>\<v>\<e>\<r> ?f : ?T \<mapsto> ?T' \<w>\<i>\<t>\<h> \<g>\<e>\<t>\<t>\<e>\<r> ?h \<s>\<e>\<t>\<t>\<e>\<r> ?s \<i>\<n> ?D \<Longrightarrow>
+  \<m>\<a>\<p> ?g \<otimes>\<^sub>f ?r : \<m>\<e>\<m>-\<c>\<o>\<e>\<r>\<c>\<e>[?TY] ?Ta \<^emph>[?C\<^sub>R] ?R \<mapsto> \<m>\<e>\<m>-\<c>\<o>\<e>\<r>\<c>\<e>[?TYa] ?Tb \<^emph>[?C\<^sub>R] ?R' \<o>\<v>\<e>\<r> ?f : ?T \<mapsto> ?T' \<w>\<i>\<t>\<h> \<g>\<e>\<t>\<t>\<e>\<r> ?h \<s>\<e>\<t>\<t>\<e>\<r> ?s \<i>\<n> ?D \<close>
+
+thm \<phi>mapToA_refl'
+thm Guided_Mem_Coercion.elim_map[where \<phi>=\<open>\<lambda>x. x\<close>, simplified, OF \<phi>mapToA_refl', \<phi>reason %mapToA_mem_coerce_end]
 
 
 subsection \<open>Auxiliary Simplification\<close>
